StrataGenerators/HasTypeAGenOpsConsistent.lean
@@ -208,7 +208,8 @@ theorem genLExprBase_opsConsistentR (F : @Factory LExprParams') (fctx : FVarCtx)
     replace he : e ∈ SetGen.support (genLExprBase (G := SetGen.Set) fctx (factoryOps F) tvars bctx 0 (.arrow τ₁ τ₂)) := by
       rw [genLExprBase.eq_def]; exact he
     rw [norm_arrow'] at he
-    simp only [genLExprBase, pick_mem_iff, mem_support_iff, SetGen.mem_dite, bot_mem_iff] at he
+    simp only [genLExprBase, mem_oneOf_iff, mem_support_oneOf_iff, List.mem_cons, List.not_mem_nil,
+      or_false, exists_eq_or_imp, exists_eq_left, pick_mem_iff, mem_support_iff, SetGen.mem_dite, bot_mem_iff] at he
     rcases he with (⟨_, h⟩ | ⟨_, h⟩) | ((⟨hf, h⟩ | ⟨_, h⟩) | (⟨_, h⟩ | ⟨_, h⟩))
     · exact pickBVar_mem_opsConsistentR F bctx (.arrow τ₁ τ₂) h
     · exact h.elim
@@ -220,7 +221,8 @@ theorem genLExprBase_opsConsistentR (F : @Factory LExprParams') (fctx : FVarCtx)
     replace he : e ∈ SetGen.support (genLExprBase (G := SetGen.Set) fctx (factoryOps F) tvars bctx 0 .bool) := by
       rw [genLExprBase.eq_def]; exact he
     rw [norm_bool'] at he
-    simp only [genLExprBase, pick_mem_iff, mem_support_iff, SetGen.mem_dite] at he
+    simp only [genLExprBase, mem_oneOf_iff, mem_support_oneOf_iff, List.mem_cons, List.not_mem_nil,
+      or_false, exists_eq_or_imp, exists_eq_left, pick_mem_iff, mem_support_iff, SetGen.mem_dite] at he
     rcases he with (rfl | rfl) | ((⟨_, h⟩ | ⟨_, rfl | rfl⟩) | ((⟨hf, h⟩ | ⟨_, rfl | rfl⟩) | (⟨_, h⟩ | ⟨_, rfl | rfl⟩)))
     · exact .const
     · exact .const
@@ -237,7 +239,8 @@ theorem genLExprBase_opsConsistentR (F : @Factory LExprParams') (fctx : FVarCtx)
     replace he : e ∈ SetGen.support (genLExprBase (G := SetGen.Set) fctx (factoryOps F) tvars bctx 0 .int) := by
       rw [genLExprBase.eq_def]; exact he
     rw [norm_int'] at he
-    simp only [genLExprBase, pick_mem_iff, SetGen.Set.mem_bind, SetGen.Set.mem_pure,
+    simp only [genLExprBase, mem_oneOf_iff, mem_support_oneOf_iff, List.mem_cons, List.not_mem_nil,
+      or_false, exists_eq_or_imp, exists_eq_left, pick_mem_iff, SetGen.Set.mem_bind, SetGen.Set.mem_pure,
       mem_support_iff, SetGen.mem_dite] at he
     rcases he with (⟨k, _, rfl⟩ | ⟨k, _, rfl⟩) | ((⟨_, h⟩ | ⟨_, ⟨k, _, rfl⟩ | ⟨k, _, rfl⟩⟩) | ((⟨hf, h⟩ | ⟨_, ⟨k, _, rfl⟩ | ⟨k, _, rfl⟩⟩) | (⟨_, h⟩ | ⟨_, ⟨k, _, rfl⟩ | ⟨k, _, rfl⟩⟩)))
     · exact .const
@@ -255,7 +258,8 @@ theorem genLExprBase_opsConsistentR (F : @Factory LExprParams') (fctx : FVarCtx)
     replace he : e ∈ SetGen.support (genLExprBase (G := SetGen.Set) fctx (factoryOps F) tvars bctx 0 .string) := by
       rw [genLExprBase.eq_def]; exact he
     rw [norm_string'] at he
-    simp only [genLExprBase, pick_mem_iff, SetGen.Set.mem_bind, SetGen.Set.mem_pure,
+    simp only [genLExprBase, mem_oneOf_iff, mem_support_oneOf_iff, List.mem_cons, List.not_mem_nil,
+      or_false, exists_eq_or_imp, exists_eq_left, pick_mem_iff, SetGen.Set.mem_bind, SetGen.Set.mem_pure,
       mem_support_iff, SetGen.mem_dite] at he
     rcases he with ⟨k, _, rfl⟩ | ((⟨_, h⟩ | ⟨_, ⟨k, _, rfl⟩⟩) | ((⟨hf, h⟩ | ⟨_, ⟨k, _, rfl⟩⟩) | (⟨_, h⟩ | ⟨_, ⟨k, _, rfl⟩⟩)))
     · exact .const
@@ -269,7 +273,8 @@ theorem genLExprBase_opsConsistentR (F : @Factory LExprParams') (fctx : FVarCtx)
     replace he : e ∈ SetGen.support (genLExprBase (G := SetGen.Set) fctx (factoryOps F) tvars bctx 0 .real) := by
       rw [genLExprBase.eq_def]; exact he
     rw [norm_real'] at he
-    simp only [genLExprBase, pick_mem_iff, SetGen.Set.mem_bind, SetGen.Set.mem_pure,
+    simp only [genLExprBase, mem_oneOf_iff, mem_support_oneOf_iff, List.mem_cons, List.not_mem_nil,
+      or_false, exists_eq_or_imp, exists_eq_left, pick_mem_iff, SetGen.Set.mem_bind, SetGen.Set.mem_pure,
       mem_support_iff, SetGen.mem_dite] at he
     rcases he with (⟨num, _, den, _, rfl⟩ | ⟨num, _, den, _, rfl⟩) | ((⟨_, h⟩ | ⟨_, (⟨num, _, den, _, rfl⟩ | ⟨num, _, den, _, rfl⟩)⟩) | ((⟨hf, h⟩ | ⟨_, (⟨num, _, den, _, rfl⟩ | ⟨num, _, den, _, rfl⟩)⟩) | (⟨_, h⟩ | ⟨_, (⟨num, _, den, _, rfl⟩ | ⟨num, _, den, _, rfl⟩)⟩)))
     · exact .const
@@ -286,7 +291,8 @@ theorem genLExprBase_opsConsistentR (F : @Factory LExprParams') (fctx : FVarCtx)
   case h_13 n =>
     replace he : e ∈ SetGen.support (genLExprBase (G := SetGen.Set) fctx (factoryOps F) tvars bctx 0 (.bitvec n)) := by
       rw [genLExprBase.eq_def]; exact he
-    simp only [genLExprBase, pick_mem_iff, SetGen.Set.mem_bind, SetGen.Set.mem_pure,
+    simp only [genLExprBase, mem_oneOf_iff, mem_support_oneOf_iff, List.mem_cons, List.not_mem_nil,
+      or_false, exists_eq_or_imp, exists_eq_left, pick_mem_iff, SetGen.Set.mem_bind, SetGen.Set.mem_pure,
       mem_support_iff, SetGen.mem_dite] at he
     rcases he with ⟨k, _, rfl⟩ | ((⟨_, h⟩ | ⟨_, ⟨k, _, rfl⟩⟩) | ((⟨hf, h⟩ | ⟨_, ⟨k, _, rfl⟩⟩) | (⟨_, h⟩ | ⟨_, ⟨k, _, rfl⟩⟩)))
     · exact .const
@@ -562,7 +568,8 @@ theorem genLExprBase_opsConsistentR (F : @Factory LExprParams') (fctx : FVarCtx)
   case h_7 name =>
     replace he : e ∈ SetGen.support (genLExprBase (G := SetGen.Set) fctx (factoryOps F) tvars bctx 0 (.ftvar name)) := by
       rw [genLExprBase.eq_def]; exact he
-    simp only [genLExprBase, pick_mem_iff, mem_support_iff, SetGen.mem_dite,
+    simp only [genLExprBase, mem_oneOf_iff, mem_support_oneOf_iff, List.mem_cons, List.not_mem_nil,
+      or_false, exists_eq_or_imp, exists_eq_left, pick_mem_iff, mem_support_iff, SetGen.mem_dite,
                bot_mem_iff] at he
     rcases he with (⟨_, h⟩ | ⟨_, ⟨hf, h⟩ | ⟨_, ⟨_, h⟩ | ⟨_, h⟩⟩⟩) |
       ((⟨hf, h⟩ | ⟨_, ⟨_, h⟩ | ⟨_, ⟨_, h⟩ | ⟨_, h⟩⟩⟩) |
@@ -628,7 +635,8 @@ theorem genLExprBase_opsConsistentR (F : @Factory LExprParams') (fctx : FVarCtx)
   case h_15 =>
     replace he : e ∈ SetGen.support (genLExprBase (G := SetGen.Set) fctx (factoryOps F) tvars bctx 0 .regex) := by
       rw [genLExprBase.eq_def]; exact he
-    simp only [genLExprBase, pick_mem_iff, mem_support_iff, SetGen.mem_dite,
+    simp only [genLExprBase, mem_oneOf_iff, mem_support_oneOf_iff, List.mem_cons, List.not_mem_nil,
+      or_false, exists_eq_or_imp, exists_eq_left, pick_mem_iff, mem_support_iff, SetGen.mem_dite,
                bot_mem_iff] at he
     rcases he with (⟨_, h⟩ | ⟨_, ⟨hf, h⟩ | ⟨_, ⟨_, h⟩ | ⟨_, h⟩⟩⟩) |
       ((⟨hf, h⟩ | ⟨_, ⟨_, h⟩ | ⟨_, ⟨_, h⟩ | ⟨_, h⟩⟩⟩) |
@@ -694,7 +702,8 @@ theorem genLExprBase_opsConsistentR (F : @Factory LExprParams') (fctx : FVarCtx)
   case h_17 τ₁ τ₂ =>
     replace he : e ∈ SetGen.support (genLExprBase (G := SetGen.Set) fctx (factoryOps F) tvars bctx 0 (.map τ₁ τ₂)) := by
       rw [genLExprBase.eq_def]; exact he
-    simp only [genLExprBase, pick_mem_iff, mem_support_iff, SetGen.mem_dite,
+    simp only [genLExprBase, mem_oneOf_iff, mem_support_oneOf_iff, List.mem_cons, List.not_mem_nil,
+      or_false, exists_eq_or_imp, exists_eq_left, pick_mem_iff, mem_support_iff, SetGen.mem_dite,
                bot_mem_iff] at he
     rcases he with (⟨_, h⟩ | ⟨_, ⟨hf, h⟩ | ⟨_, ⟨_, h⟩ | ⟨_, h⟩⟩⟩) |
       ((⟨hf, h⟩ | ⟨_, ⟨_, h⟩ | ⟨_, ⟨_, h⟩ | ⟨_, h⟩⟩⟩) |
@@ -760,7 +769,8 @@ theorem genLExprBase_opsConsistentR (F : @Factory LExprParams') (fctx : FVarCtx)
   case h_19 τ =>
     replace he : e ∈ SetGen.support (genLExprBase (G := SetGen.Set) fctx (factoryOps F) tvars bctx 0 (.seq τ)) := by
       rw [genLExprBase.eq_def]; exact he
-    simp only [genLExprBase, pick_mem_iff, mem_support_iff, SetGen.mem_dite,
+    simp only [genLExprBase, mem_oneOf_iff, mem_support_oneOf_iff, List.mem_cons, List.not_mem_nil,
+      or_false, exists_eq_or_imp, exists_eq_left, pick_mem_iff, mem_support_iff, SetGen.mem_dite,
                bot_mem_iff] at he
     rcases he with (⟨_, h⟩ | ⟨_, ⟨hf, h⟩ | ⟨_, ⟨_, h⟩ | ⟨_, h⟩⟩⟩) |
       ((⟨hf, h⟩ | ⟨_, ⟨_, h⟩ | ⟨_, ⟨_, h⟩ | ⟨_, h⟩⟩⟩) |
@@ -1220,14 +1230,8 @@ theorem genLExpr_opsConsistentR (F : @Factory LExprParams') (fctx : FVarCtx) (pc
     exact genLExprBase_opsConsistentR F fctx tvars bctx depth τ e he
   · -- monomorphic Indir
     simp only [SetGen.Set.mem_bind, SetGen.Set.mem_pure] at he
-    obtain ⟨idx, ⟨_, hidx_hi⟩, args, hargs, rfl⟩ := he
-    have hlt : idx.down.val < (findOpsInCtx (factoryOps F) τ).length := by omega
-    have hentry_mem : (findOpsInCtx (factoryOps F) τ).getD idx.down.val ("", []) ∈
-        findOpsInCtx (factoryOps F) τ := by
-      have heq : (findOpsInCtx (factoryOps F) τ).getD idx.down.val ("", []) =
-          (findOpsInCtx (factoryOps F) τ)[idx.down.val] := by
-        simp [List.getD, List.getElem?_eq_getElem hlt]
-      rw [heq]; exact List.getElem_mem hlt
+    obtain ⟨⟨name, argTys⟩, hentry_mem, args, hargs, rfl⟩ := he
+    rw [← mem_support_iff, mem_support_elements_iff] at hentry_mem
     apply mkApps_opsConsistentR
     · exact indir_op_opsConsistentR F τ _ _ hentry_mem
     · exact mapM_genLExprBase_opsConsistentR F fctx tvars bctx depth _ args hargs
@@ -1338,14 +1342,8 @@ theorem genLExpr_opsConsistentR_nil (F : @Factory LExprParams') (fctx : FVarCtx)
   rcases he with ⟨hpos, he | (he | he)⟩ | ⟨_, he | he⟩
   · exact genLExprBase_opsConsistentR F fctx tvars bctx depth τ e he
   · simp only [SetGen.Set.mem_bind, SetGen.Set.mem_pure] at he
-    obtain ⟨idx, ⟨_, hidx_hi⟩, args, hargs, rfl⟩ := he
-    have hlt : idx.down.val < (findOpsInCtx (factoryOps F) τ).length := by omega
-    have hentry_mem : (findOpsInCtx (factoryOps F) τ).getD idx.down.val ("", []) ∈
-        findOpsInCtx (factoryOps F) τ := by
-      have heq : (findOpsInCtx (factoryOps F) τ).getD idx.down.val ("", []) =
-          (findOpsInCtx (factoryOps F) τ)[idx.down.val] := by
-        simp [List.getD, List.getElem?_eq_getElem hlt]
-      rw [heq]; exact List.getElem_mem hlt
+    obtain ⟨⟨name, argTys⟩, hentry_mem, args, hargs, rfl⟩ := he
+    rw [← mem_support_iff, mem_support_elements_iff] at hentry_mem
     apply mkApps_opsConsistentR
     · exact indir_op_opsConsistentR F τ _ _ hentry_mem
     · exact mapM_genLExprBase_opsConsistentR F fctx tvars bctx depth _ args hargs
